move non-example defns from Merge.v, MergePartial.v to Combinators.v

theories/Merge.v
@@ -7,7 +7,7 @@ From ITree Require Export ITree ITreeFacts Eq.Rutt Props.Finite.
 From Paco Require Import paco.
 From Coq Require Export Eqdep EqdepFacts.
 Require Import Lia.
-Require Export Refinement.
+Require Export Refinement Combinators.
 
 Import Monads.
 Import MonadNotation.
@@ -16,11 +16,9 @@ Locate MonadNotation.
 Open Scope list_scope.
 
 Locate Permutation.
-(*
-Inductive sorted : list nat -> Prop :=
-  | sorted_nil : sorted nil
-  | sorted_singleton x : sorte
-. *)
+
+Opaque assume_spec.
+Opaque assert_spec.
 
 
 Inductive sorted : list nat -> Prop :=
@@ -60,19 +58,6 @@ Proof.
       ) as f. auto.
 Qed.
 
-(*rec_fix*)
-(* call *)
-Definition call_spec {E A B} (a : A) : itree_spec (callE A B +' E) B :=
-  ITree.trigger (Spec_vis (inl1 (Call a))).
-
-Definition rec_spec {E A B} (body : A -> itree_spec (callE A B +' E) B) (a : A) :
-  itree_spec E B :=
-  mrec_spec (calling' body) (Call a).
-
-Definition rec_fix_spec {E A B}
-(body : (A -> itree_spec (callE A B +' E) B) ->
-        A -> itree_spec (callE A B +' E) B)  :
-  A -> itree_spec E B := rec_spec (body call_spec).
 
 Definition halve {E} : list nat -> itree_spec E (list nat * list nat) :=
     rec_fix_spec (fun halve_rec l =>
@@ -82,148 +67,6 @@ Definition halve {E} : list nat -> itree_spec E (list nat * list nat) :=
                | nil => Ret ( nil , nil ) end
 
 ).
-
-Definition assert_spec {E} (P : Type) : itree_spec E unit :=
-  trigger (@Spec_exists E P);; Ret tt.
-
-Lemma padded_assert_pad_elim {E1 E2} RPre RPost R1 R2 RR P
-      (phi : itree_spec E1 R1) (kphi : unit -> itree_spec E2 R2) :
-  P -> padded_refines RPre RPost RR phi (kphi tt) ->
-  padded_refines RPre RPost RR phi (ITree.bind (assert_spec P) kphi).
-Proof.
-  intros. setoid_rewrite bind_trigger.
-  unfold padded_refines in *. rewrite pad_bind, pad_vis.
-  setoid_rewrite pad_ret. rewrite bind_vis. setoid_rewrite bind_tau.
-  setoid_rewrite bind_ret_l. pstep. constructor. auto. constructor. pstep_reverse.
-Qed.
-
-Lemma padded_assert_pad_eliml {E1 E2} RPre RPost R1 R2 RR P
-      (phi : itree_spec E1 R1) (kphi : unit -> itree_spec E2 R2) :
-  (P -> padded_refines RPre RPost RR (kphi tt) phi) ->
-  padded_refines RPre RPost RR (ITree.bind (assert_spec P) kphi) phi.
-Proof.
-  intros. setoid_rewrite bind_trigger.
-  unfold padded_refines in *. rewrite pad_bind, pad_vis.
-  setoid_rewrite pad_ret. rewrite bind_vis. setoid_rewrite bind_tau.
-  setoid_rewrite bind_ret_l. pstep. constructor.
-  intros HP. specialize (H HP). constructor. pstep_reverse.
-Qed.
-
-
-Definition assume_spec {E} (P : Type) : itree_spec E unit :=
-  trigger (@Spec_forall E P);; Ret tt.
-
-Lemma padded_assume_pad_elim {E1 E2} RPre RPost R1 R2 RR P
-      (phi : itree_spec E1 R1) (kphi : unit -> itree_spec E2 R2) :
-  (P -> padded_refines RPre RPost RR phi (kphi tt)) ->
-  padded_refines RPre RPost RR phi (ITree.bind (assume_spec P) kphi).
-Proof.
-  intros. setoid_rewrite bind_trigger.
-  unfold padded_refines in *. rewrite pad_bind, pad_vis.
-  setoid_rewrite pad_ret. rewrite bind_vis. setoid_rewrite bind_tau.
-  setoid_rewrite bind_ret_l. pstep. constructor.
-  intros HP. specialize (H HP). constructor. pstep_reverse.
-Qed.
-
-Lemma padded_assume_pad_eliml {E1 E2} RPre RPost R1 R2 RR P
-      (phi : itree_spec E1 R1) (kphi : unit -> itree_spec E2 R2) :
-  P -> padded_refines RPre RPost RR (kphi tt) phi ->
-  padded_refines RPre RPost RR (ITree.bind (assume_spec P) kphi) phi.
-Proof.
-  intros. setoid_rewrite bind_trigger.
-  unfold padded_refines in *. rewrite pad_bind, pad_vis.
-  setoid_rewrite pad_ret. rewrite bind_vis. setoid_rewrite bind_tau.
-  setoid_rewrite bind_ret_l. pstep. constructor. auto. constructor. pstep_reverse.
-Qed.
-
-Opaque assume_spec.
-
-Definition exists_spec {E} (T : Type) : itree_spec E T :=
-  trigger (@Spec_exists E T).
-
-
-(**)
-Lemma exists_spec_elim {E1 E2} S1 R2 S2 RPre RPost RR (phi : itree_spec E1 S1)
-      (kphi : R2 -> itree_spec E2 S2) r :
-  refines RPre RPost RR phi (kphi r) ->
-  refines RPre RPost RR phi (ITree.bind (exists_spec R2) kphi).
-Proof.
-  intros. unfold exists_spec. setoid_rewrite bind_trigger.
-  pstep. econstructor. pstep_reverse.
-Qed.
-
-Opaque assert_spec.
-
-(*maybe there is a simpler way to derive this proof from the previous one*)
-Lemma padded_exists_spec_elim {E1 E2} S1 R2 S2 RPre RPost RR (phi : itree_spec E1 S1)
-      (kphi : R2 -> itree_spec E2 S2) r :
-  padded_refines RPre RPost RR phi (kphi r) ->
-  padded_refines RPre RPost RR phi (ITree.bind (exists_spec R2) kphi).
-Proof.
-  intros.  unfold padded_refines in *. rewrite pad_bind. setoid_rewrite pad_vis.
-  rewrite bind_vis.
-  setoid_rewrite pad_ret. setoid_rewrite bind_tau. setoid_rewrite bind_ret_l.
-  pstep. econstructor. Unshelve. all : auto. constructor. pstep_reverse.
-Qed.
-
-Lemma padded_exists_spec_eliml {E1 E2} S1 R2 S2 RPre RPost RR (phi : itree_spec E1 S1)
-      (kphi : R2 -> itree_spec E2 S2) :
-  (forall r, padded_refines RPre RPost RR (kphi r) phi) ->
-  padded_refines RPre RPost RR (ITree.bind (exists_spec R2) kphi) phi .
-Proof.
-  intros.  unfold padded_refines in *. rewrite pad_bind. setoid_rewrite pad_vis.
-  rewrite bind_vis.
-  setoid_rewrite pad_ret. setoid_rewrite bind_tau. setoid_rewrite bind_ret_l.
-  pstep. econstructor. intros. constructor. pstep_reverse. apply H.
-Qed.
-
-Ltac existssr a := apply padded_exists_spec_elim with (r := a).
-
-Ltac eexistssr := eapply padded_exists_spec_elim.
-
-Ltac existssl := apply padded_exists_spec_eliml.
-
-Ltac assumesr := apply padded_assume_pad_elim.
-Ltac assumesl := apply padded_assume_pad_eliml.
-Ltac assertsr := apply padded_assert_pad_elim.
-Ltac assertsl := apply padded_assert_pad_eliml.
-
-Definition forall_spec {E} (T : Type) : itree_spec E T :=
-  trigger (@Spec_forall E T).
-
-Lemma forall_spec_elim {E1 E2} S1 R2 S2 RPre RPost RR (phi : itree_spec E1 S1)
-      (kphi : R2 -> itree_spec E2 S2) :
-  (forall r, refines RPre RPost RR phi (kphi r)) ->
-  refines RPre RPost RR phi (ITree.bind (forall_spec R2) kphi).
-Proof.
-  intros. unfold forall_spec. rewrite bind_trigger.
-  pstep. constructor. intros. pstep_reverse. apply H.
-Qed.
-
-Lemma padded_forall_spec_elim {E1 E2} S1 R2 S2 RPre RPost RR (phi : itree_spec E1 S1)
-      (kphi : R2 -> itree_spec E2 S2):
-  (forall r, padded_refines RPre RPost RR phi (kphi r)) ->
-  padded_refines RPre RPost RR phi (ITree.bind (forall_spec R2) kphi).
-Proof.
-  intros.  unfold padded_refines in *. rewrite pad_bind. setoid_rewrite pad_vis.
-  rewrite bind_vis.
-  setoid_rewrite pad_ret. setoid_rewrite bind_tau. setoid_rewrite bind_ret_l.
-  pstep. constructor. intros.  constructor. pstep_reverse.
-  apply H.
-Qed.
-
-Lemma padded_forall_spec_eliml {E1 E2} S1 R2 S2 RPre RPost RR (phi : itree_spec E1 S1)
-      (kphi : R2 -> itree_spec E2 S2) r:
-  padded_refines RPre RPost RR (kphi r) phi ->
-  padded_refines RPre RPost RR (ITree.bind (forall_spec R2) kphi) phi.
-Proof.
-  intros.  unfold padded_refines in *. rewrite pad_bind. setoid_rewrite pad_vis.
-  rewrite bind_vis.
-  setoid_rewrite pad_ret. setoid_rewrite bind_tau. setoid_rewrite bind_ret_l.
-  pstep. econstructor. constructor. pstep_reverse.
-Qed.
-
-
 
 Definition halve_spec {E} (l : list nat) : itree_spec E (list nat * list nat) :=
   l1 <- exists_spec (list nat);;
@@ -285,123 +128,6 @@ Definition sort_spec {E} (l : list nat) : itree_spec E (list nat) :=
   assert_spec (Permutation l l');;
   assert_spec (sorted l');;
   Ret l'.
-
-
-Definition padded_refines_eq {E R1 R2} RR (phi1 : itree_spec E R1) (phi2 : itree_spec E R2) :=
-  padded_refines eqPreRel eqPostRel RR phi1 phi2.
-
-Instance proper_leq : Proper (le ==> le ==> le) plus.
-Proof.
-  repeat intro. lia. Qed.
-
-Global Instance padded_refines_eq_refl {E R} : Reflexive (@padded_refines_eq E R R eq).
-Proof.
-  red. intros. unfold padded_refines_eq, padded_refines. apply refl_refines; auto.
-  - red. intros. constructor.
-  - red. intros. inv H. inj_existT. subst. auto.
-  - apply pad_is_padded.
-Qed.
-
-Global Instance refines_proper_bind E R S :
-  Proper (@padded_refines_eq E R R eq ==> pointwise_relation _ (padded_refines_eq eq) ==> @padded_refines_eq E S S eq) ITree.bind.
-Proof.
-  repeat intro. subst. unfold padded_refines_eq in *. eapply padded_refines_bind; eauto.
-  intros; subst. auto.
-Qed.
-
-Global Instance refines_proper_subst E R S (k : R -> itree_spec E S) :
-  Proper (@padded_refines_eq E R R eq ==> padded_refines_eq eq) (ITree.subst k).
-Proof.
-  repeat intro. eapply refines_proper_bind. auto. intro. reflexivity.
-Qed.
-
-Global Instance refines_proper_bind_eq E R S :
-  Proper (@padded_refines_eq E R R eq ==> eq ==> @padded_refines_eq E S S eq) ITree.bind.
-Proof.
-  repeat intro. eapply refines_proper_bind. auto. subst. intro. reflexivity.
-Qed.
-
-Lemma eqPreRel_eq_type E A B (ea : E A) (eb : E B) : eqPreRel A B ea eb -> A = B.
-Proof.
-  intros. inv H. auto.
-Qed.
-
-Lemma eqPreRel_eq E A (e1 : E A) (e2 : E A) : eqPreRel A A e1 e2 -> e1 = e2.
-Proof.
-  intros. inv H. inj_existT. subst. auto.
-Qed.
-
-Lemma eqPostRel_eq_type E A B (ea : E A) (eb : E B) a b : eqPostRel A B ea eb a b -> A = B.
-Proof.
-  intros. inv H. auto.
-Qed.
-
-Lemma eqPostRel_eq E A (e1 : E A) (e2 : E A) a1 a2 : eqPostRel A A e1 e2 a1 a2 -> e1 = e2 /\ a1 = a2.
-Proof.
-  intros. inv H. inj_existT. subst. auto.
-Qed.
-
-Ltac eqPreRel_inv H := apply eqPreRel_eq_type in H as ?H; subst; apply eqPreRel_eq in H; subst.
-Ltac eqPostRel_inv H := apply eqPostRel_eq_type in H as ?H; subst; apply eqPostRel_eq in H as [?H ?H]; subst.
-
-Global Instance padded_refines_eq_trans {E R} : Transitive (@padded_refines_eq E R R eq).
-Proof.
-  intros phi1 phi2 phi3 Hphi12 Hphi23. unfold padded_refines_eq, padded_refines in *.
-  eapply refines_monot; try eapply refinesTrans; eauto with solve_padded; try apply pad_is_padded.
-  - intros A B ea eb PR. assert (A = B). inv PR. inv H3. inv H4. auto. subst.
-    assert (ea = eb). inv PR. inj_existT.
-    subst. assert (B = B0). inv H3. auto. subst. inv H4. inj_existT. subst. inv H3. inj_existT.
-    subst. auto. subst. constructor.
-  - intros.
-    assert (A = B). inv PR. auto. subst. assert (ea = eb). inv PR. inj_existT. subst. auto.
-    subst. constructor. intros. destruct H. assert (x0 = x1). inv PR. inj_existT. subst. auto.
-    subst. assert (B = B0). inv H. auto. subst. exists x1.
-    assert (e2 = eb). inv H. inj_existT. subst. auto. subst. repeat constructor.
-  - intros. inv PR. auto.
-Qed.
-
-Global Instance refines_proper_interp_mrec_spec E D R :
-  Proper ((fun ctx1 ctx2 => forall T d, padded_refines_eq  eq (ctx1 T d) (ctx2 T d)) ==> @padded_refines_eq (D +' E) R R eq ==> @padded_refines_eq E R R eq)
-         (fun ctx => @interp_mrec_spec D E ctx R).
-Proof.
-  repeat intro. subst. unfold padded_refines_eq in *.
-  eapply padded_refines_interp_mrec with (RPreInv := eqPreRel) (RPostInv := eqPostRel) ; eauto.
-  - intros.
-    eqPreRel_inv H1.
-    eapply refines_monot; try eapply H.
-    + intros.  eqPreRel_inv PR. destruct x2; repeat constructor.
-    + intros. inv PR; inj_existT; subst; eqPostRel_inv H7; constructor.
-    + intros. subst. constructor.
-  - eapply refines_monot; try eapply H0.
-    + intros. eqPreRel_inv PR. destruct x2; repeat constructor.
-    + intros. inv PR; inj_existT; subst; eqPostRel_inv H7; constructor.
-    + auto.
-Qed.
-
-Global Instance refines_proper_interp_mrec_spec_eq E D R :
-  Proper (eq ==> @padded_refines_eq (D +' E) R R eq ==> @padded_refines_eq E R R eq)
-         (fun ctx => @interp_mrec_spec D E ctx R).
-Proof.
-  repeat intro.
-  apply refines_proper_interp_mrec_spec; auto.
-  intros. subst. reflexivity.
-Qed.
-
-
-(*
-Global Instance padded_refines_eq_bind_proper  E1 E2 RPre RPost R1 R2 RR :
-  Proper (padded_refines_eq eq ==> eq ==> @padded_refines E1 E2 R1 R2 RPre RPost RR) ITree.bind.
-*)
-(*from there there is a bit more *)
-
-(*need at least bind and ret rules for interp_mrec_spec *)
-
-Lemma interp_mrec_ret :
-  forall {D E : Type -> Type} (ctx : forall T : Type, D T -> itree (D +' E) T) R (r :R),
-    interp_mrec ctx (Ret r) ≅ Ret r.
-Proof.
-  intros. setoid_rewrite unfold_iter. cbn. rewrite bind_ret_l. reflexivity.
-Qed.
 
 
 Instance perm_eq A : Equivalence (@Permutation A).
@@ -523,53 +249,3 @@ Section strong_list_ind.
   Qed.
 
 End strong_list_ind.
-
-
-Lemma interp_mrec_exists_spec E D T (ctx : forall T, D T -> itree_spec (D +' E) T) :
-  interp_mrec_spec ctx (exists_spec T) ≈ exists_spec T.
-Proof.
-  setoid_rewrite interp_mrec_spec'_exists.
-  cbn. apply eqit_Vis. intros.  pstep. red. cbn. constructor. auto.
-Qed.
-
-Lemma interp_mrec_forall_spec E D T (ctx : forall T, D T -> itree_spec (D +' E) T) :
-  interp_mrec_spec ctx (forall_spec T) ≈ forall_spec T.
-Proof.
-  setoid_rewrite interp_mrec_spec'_forall.
-  cbn. apply eqit_Vis. intros.  pstep. red. cbn. constructor. auto.
-Qed.
-
-Lemma interp_mrec_spec_assume E D T (ctx : forall T, D T -> itree_spec (D +' E) T) :
-  interp_mrec_spec ctx (assume_spec T) ≈ assume_spec T.
-Proof.
-  Transparent assume_spec. unfold assume_spec.
-  cbn. setoid_rewrite interp_mrec_spec_bind.
-  setoid_rewrite interp_mrec_spec'_forall. rewrite bind_vis, bind_trigger.
-  apply eqit_Vis. intros. setoid_rewrite interp_mrec_spec_ret. rewrite bind_ret_l.
-  reflexivity.
-  Opaque assume_spec.
-Qed.
-
-Lemma interp_mrec_spec_assert E D T (ctx : forall T, D T -> itree_spec (D +' E) T) :
-  interp_mrec_spec ctx (assert_spec T) ≈ assert_spec T.
-Proof.
-  Transparent assert_spec. unfold assert_spec.
-  cbn. setoid_rewrite interp_mrec_spec_bind.
-  setoid_rewrite interp_mrec_spec'_exists. rewrite bind_vis, bind_trigger.
-  apply eqit_Vis. intros. setoid_rewrite interp_mrec_spec_ret. rewrite bind_ret_l.
-  reflexivity.
-  Opaque assert_spec.
-Qed.
-
-Ltac normalize_interp_mrec_spec :=
-  match goal with
-  | |- context [ITree.bind (ITree.bind ?t ?k1) ?k2 ] => setoid_rewrite bind_bind
-  | |- context [interp_mrec_spec ?ctx (ITree.bind ?t ?k) ] => setoid_rewrite interp_mrec_spec_bind
-  | |- context [interp_mrec_spec ?ctx (exists_spec ?T) ] => setoid_rewrite interp_mrec_exists_spec
-  | |- context [interp_mrec_spec ?ctx (forall_spec ?T) ] => setoid_rewrite interp_mrec_forall_spec
-  | |- context [interp_mrec_spec ?ctx (assert_spec ?T) ] => setoid_rewrite interp_mrec_spec_assert
-  | |- context [interp_mrec_spec ?ctx (assume_spec ?T) ] => setoid_rewrite interp_mrec_spec_assume
-  end.
-
-Variant Err : Type -> Type :=
-  | throw : Err void.
