theories/MergePartial.v
@@ -5,7 +5,7 @@ From ITree Require Export ITree ITreeFacts Eq.Rutt Props.Finite.
 From Paco Require Import paco.
 From Coq Require Export Eqdep EqdepFacts Logic.Classical.
 Require Import Lia.
-Require Export Refinement Merge ConvergentRefinement ConcreteRefinement.
+Require Export Refinement Combinators ConvergentRefinement ConcreteRefinement Automation Merge.
 
 Import Monads.
 Import MonadNotation.
@@ -13,33 +13,6 @@ Local Open Scope monad_scope.
 
 Open Scope list_scope.
 
-
-Lemma or_spec_l E1 E2 RPre RPost R1 R2 RR (t1 t2 : itree_spec E1 R1) (t3 : itree_spec E2 R2) :
-  @padded_refines E1 E2 R1 R2 RPre RPost RR t1 t3 ->
-  @padded_refines E1 E2 R1 R2 RPre RPost RR t2 t3 ->
-  @padded_refines E1 E2 R1 R2 RPre RPost RR (or_spec t1 t2) t3.
-Proof.
-  intros. unfold or_spec. unfold padded_refines in *.
-  rewrite pad_vis. pstep. constructor. intros [ | ]; constructor; pstep_reverse.
-Qed.
-
-Lemma or_spec_r E1 E2 RPre RPost R1 R2 RR (t1 : itree_spec E1 R1) (t2 t3: itree_spec E2 R2) :
-  (@padded_refines E1 E2 R1 R2 RPre RPost RR t1 t2 \/
-  @padded_refines E1 E2 R1 R2 RPre RPost RR t1 t3) ->
-  @padded_refines E1 E2 R1 R2 RPre RPost RR t1 (or_spec t2 t3).
-Proof.
-  intros. unfold or_spec. unfold padded_refines in *.
-  rewrite pad_vis. pstep.
-  destruct H.
-  - econstructor. constructor. Unshelve. all : try (apply true). pstep_reverse.
-  - econstructor. constructor. Unshelve. all : try (apply false). pstep_reverse.
-Qed.
-
-Lemma spin_bind E R S k : (@ITree.spin E R) >>= k ≅ @ITree.spin E S.
-Proof.
-  ginit. gcofix CIH. gstep. red. cbn. constructor.
-  gfinal. eauto.
-Qed.
 
 Lemma and_or_spec E R (t1 t2 : itree_spec E R) :
   padded_refines_eq eq (and_spec t1 t2) (or_spec t1 t2).
@@ -51,20 +24,6 @@ Proof.
   enough (padded_refines_eq eq t1 t1). auto. reflexivity.
 Qed.
 
-Fixpoint trepeat {E R} (n : nat) (t : itree E R) : itree E unit :=
-  match n with
-  | 0 => Ret tt
-  | S m => t;; trepeat m t end.
-
-Lemma trepeat_Sn E R (n : nat) (t : itree E R) :
-  trepeat (S n) t ≅ t;; trepeat n t.
-Proof.
-  apply eqit_bind; reflexivity.
-Qed.
-
-Lemma trepeat_0 E R (t : itree E R) :
-  trepeat 0 t ≅ Ret tt.
-Proof. reflexivity. Qed.
 
 Definition halve_spec_fix {E} : list nat -> itree_spec E (list nat * list nat) :=
   rec_fix_spec (fun halve_spec_rec l =>
@@ -72,26 +31,6 @@ Definition halve_spec_fix {E} : list nat -> itree_spec E (list nat * list nat) :
                   trepeat n ( l' <- exists_spec (list nat);; halve_spec_rec l' );;
                   halve_spec l
                ).
-
-
-Theorem padded_refines_ret E1 E2 R1 R2 RPre RPost RR r1 r2 :
-  (RR r1 r2 : Prop) ->
-  @padded_refines E1 E2 R1 R2 RPre RPost RR (Ret r1) (Ret r2).
-Proof.
-  intros Hr. red. repeat rewrite pad_ret. pstep. constructor. auto.
-Qed.
-
-Theorem padded_refines_vis E1 E2 R1 R2 A B
-        RPre RPost RR (e1 : E1 A) (e2 : E2 B)
-        (k1 : A -> itree_spec E1 R1) (k2 : B -> itree_spec E2 R2) :
-  (RPre A B e1 e2 : Prop) ->
-  (forall a b, (RPost A B e1 e2 a b : Prop) -> padded_refines RPre RPost RR (k1 a) (k2 b)) ->
-  padded_refines RPre RPost RR (Vis (Spec_vis e1) k1) (Vis (Spec_vis e2) k2).
-Proof.
-  unfold padded_refines. setoid_rewrite pad_vis. intros.
-  pstep. constructor; auto. intros. left. pstep. constructor.
-  left. eapply H0; auto.
-Qed.
 
 Variant halve_call : forall A, callE (list nat) (list nat * list nat) A -> A -> Prop :=
   | halve_call_i (l l1 l2: list nat) :
@@ -142,432 +81,25 @@ Proof.
       cbn. repeat rewrite H0. repeat rewrite app_length. lia.
 Qed.
 
-
-Global Instance padded_refines_eq_itree E1 E2 R1 R2 RPre RPost RR
-  : Proper (eq_itree eq ==> eq_itree eq ==> impl)
-           (@padded_refines E1 E2 R1 R2 RPre RPost RR).
+Lemma auto_halve_correct' E l :
+  padded_refines_eq eq (@halve E l) (@halve_spec_fix E l).
 Proof.
-  repeat intro. assert (x ≈ y). rewrite H. reflexivity.
-  rewrite <- H2. assert (x0 ≈ y0). rewrite H0. reflexivity.
-  rewrite <- H3. auto.
+  unfold halve, halve_spec_fix, halve_spec.
+  prove_refinement.
+  - exact (a = a0).
+  - exact ((Permutation a (fst r ++ snd r)) /\
+           (length (fst r) >= length (snd r) /\ (length a > length (fst r) \/ length a <= 1))).
+  - prove_refinement_continue.
+    Check padded_refines_trigger_bind_r.
+    all: cbn; cbn in *.
+    all: try split; try easy; try lia.
+    + rewrite Permutation_app_comm. cbn.
+      rewrite H0. rewrite Permutation_app_comm. reflexivity.
+    + rewrite H0. repeat rewrite app_length. lia.
+    + rewrite Permutation_app_comm. cbn.
+      rewrite H0. rewrite Permutation_app_comm. reflexivity.
+    + repeat rewrite H0. repeat rewrite app_length. lia.
 Qed.
-
-Lemma interp_mrec_spec_or  (E : Type -> Type) (R : Type) (D : Type -> Type) (ctx : forall T : Type, D T -> itree_spec (D +' E) T)
-  (t1 t2 : itree_spec _ R)
-  : interp_mrec_spec ctx (or_spec t1 t2) ≅ or_spec (interp_mrec_spec ctx t1) (interp_mrec_spec ctx t2).
-Proof.
-  setoid_rewrite interp_mrec_spec'_exists. apply eqit_Vis. intros [ | ]; reflexivity.
-Qed.
-
-Lemma interp_mrec_spec_spin (E : Type -> Type) (R : Type) (D : Type -> Type) (ctx : forall T : Type, D T -> itree_spec (D +' E) T) :
-  interp_mrec_spec ctx ITree.spin ≅ @ITree.spin _ R.
-Proof.
-  pcofix CIH. pstep. red. cbn. constructor.
-  right. eauto.
-Qed.
-
-Lemma conv_ref_mrec_spin (E D : Type -> Type) (R : Type) (P : forall A : Type, D A -> Prop) :
-  @conv_ref_mrec E D R P ITree.spin.
-Proof.
-  pcofix CIH. pstep. red. cbn. constructor.
-  eauto.
-Qed.
-
-Lemma conv_ref_mrec_ret (E D : Type -> Type) (R : Type) (P : forall A : Type, D A -> Prop) r:
-  @conv_ref_mrec E D R P (Ret r).
-Proof.
-  pstep. constructor.
-Qed.
-
-Lemma conv_ref_mrec_ex (E D : Type -> Type) (R A : Type) (P : forall A : Type, D A -> Prop) k :
-  (forall a, conv_ref_mrec P (k a)) ->
-  @conv_ref_mrec E D R P (Vis (@Spec_exists _ A) k).
-Proof.
-  intros. pstep. constructor. left. apply H.
-Qed.
-
-(*should be able to generalize this to cany concrete tree *)
-Lemma or_spec_r_Ret_inv E1 E2 R1 R2 RPre RPost RR r t2 t3 :
-  @padded_refines E1 E2 R1 R2 RPre RPost RR (Ret r) (or_spec t2 t3) ->
-  padded_refines RPre RPost RR (Ret r) t2 \/ padded_refines RPre RPost RR (Ret r) t3.
-Proof.
-  intros Hor. unfold padded_refines in *. setoid_rewrite pad_ret in Hor.
-  setoid_rewrite pad_ret. setoid_rewrite pad_vis in Hor.
-  pinversion Hor. inj_existT. subst. inv H1. destruct a.
-  - left. pstep. auto.
-  - right. pstep. auto.
-Qed.
-
-Lemma conv_ref_exists_spec E R :
-  @conv_ref E R (exists_spec R).
-Proof.
-  pstep. red. cbn. constructor.
-  intros. left. pstep. constructor.
-Qed.
-
-Section SpecFix.
-  Context {A B: Type} {E : Type -> Type}.
-  Context (Pre : A -> Prop) (Post : A -> B -> Prop).
-  Context (prog : A -> itree_spec E B).
-
-  Context (Rdec : A -> A -> Prop).
-  Context (HRdec : well_founded Rdec).
-
-  Context (Hprog : forall a, isConcrete (prog a)).
-  Variant pre_call : forall C, callE A B C -> Prop :=
-    | pre_call_intro (a : A) : Pre a -> pre_call B (Call a).
-  Variant post_call : forall C, callE A B C -> C -> Prop :=
-    | post_call_intro a b : Post a b -> post_call B (Call a) b.
-
-  Definition total_spec (a : A) : itree_spec E B :=
-    assume_spec (Pre a);;
-    b <- exists_spec B;;
-    assert_spec (Post a b);;
-    Ret b.
-
-  (* better for using as a final spec *)
-  Definition partial_spec (a : A) : itree_spec E B :=
-    or_spec (total_spec a) ITree.spin.
-  (* better for syntax driven solving *)
-  (**)
-
-  Definition partial_spec_fix : A -> itree_spec E B :=
-    rec_fix_spec (fun rec a =>
-                    assume_spec (Pre a);;
-                    (
-                      n <- exists_spec nat;;
-                      trepeat n (a' <- exists_spec A;; assert_spec (Pre a');; rec a')
-                    );;
-                    b <- exists_spec B;;
-                    assert_spec (Post a b);;
-                    Ret b
-                 ).
-
-  Definition partial_spec_fix' : A -> itree_spec E B :=
-    rec_fix_spec (fun rec a =>
-                        assume_spec (Pre a);;
-                        (
-                          n <- exists_spec nat;;
-                          trepeat n (a' <- exists_spec A;; assert_spec (Pre a');; rec a')
-                        );;
-                        or_spec (
-                            b <- exists_spec B;;
-                            assert_spec (Post a b);;
-                            Ret b)
-                        ITree.spin
-                 ).
-
-
-  Definition total_spec_fix : A -> itree_spec E B :=
-    rec_fix_spec (fun rec a =>
-                    assume_spec (Pre a);;
-                    (
-                      n <- exists_spec nat;;
-                      trepeat n (a' <- exists_spec A;; assert_spec (Pre a' /\ Rdec a' a);; rec a')
-                    );;
-                    b <- exists_spec B;;
-                    assert_spec (Post a b);;
-                    Ret b
-                 ).
-
-  (* here would be a good place for proofs that partial_spec_fix' is greater than any of these
-     from there I should be able to prove that total_spec_fix
-   *)
-
-  Lemma total_spec_fix_total a : padded_refines_eq eq (total_spec_fix a) (total_spec a).
-  Proof.
-    revert a.
-    apply well_founded_ind with (R := Rdec). auto.
-    intros a Hind. unfold total_spec_fix. simpl.
-    setoid_rewrite interp_mrec_spec_bind.
-    match goal with |- context [ interp_mrec_spec ?k _ ] => set k as body end.
-    unfold total_spec. assumesr. intros Ha. setoid_rewrite interp_mrec_spec_assume.
-    assumesl. auto. rewrite bind_bind.  setoid_rewrite interp_mrec_spec_bind.
-    setoid_rewrite interp_mrec_exists_spec. existssl. intros n.
-    induction n.
-    - simpl. rewrite bind_ret_l. setoid_rewrite interp_mrec_spec_bind.
-      setoid_rewrite interp_mrec_exists_spec.
-      setoid_rewrite interp_mrec_spec_bind. setoid_rewrite interp_mrec_spec_assert.
-      setoid_rewrite interp_mrec_spec_ret. reflexivity.
-    - simpl. rewrite bind_bind. setoid_rewrite interp_mrec_spec_bind.
-      setoid_rewrite IHn. setoid_rewrite interp_mrec_spec_bind.
-      setoid_rewrite interp_mrec_exists_spec. rewrite bind_bind. existssl.
-      intros a'. setoid_rewrite interp_mrec_spec_bind.
-      setoid_rewrite interp_mrec_spec_assert. rewrite bind_bind. assertsl.
-      intros [Hprea' Hdec]. simpl.
-      assert (Htot : interp_mrec_spec body (call_spec a') ≈ total_spec_fix a').
-      { unfold total_spec_fix, rec_fix_spec, rec_spec, mrec_spec .
-        setoid_rewrite interp_mrec_spec_inl. rewrite tau_eutt. rewrite bind_ret_r.
-        reflexivity. }
-      rewrite Htot, Hind; auto. unfold total_spec.
-      setoid_rewrite bind_bind at 1. assumesl. auto.
-      setoid_rewrite bind_bind at 1. existssl. intros b.
-      setoid_rewrite bind_bind at 1. assertsl. intros. rewrite bind_ret_l. reflexivity.
-   Qed.
-
-
-    Lemma partial_spec_fix_conv_ref :
-    forall a, Pre a -> conv_ref (partial_spec_fix' a).
-  Proof.
-    intros a Ha.
-    eapply conv_ref_mrec_conv_ref with (Pre := pre_call).
-    constructor. auto.
-    intros. inv H. inj_existT. subst.
-    clear a Ha.
-    rename a0 into a. rename H2 into Ha. clear H0. cbn.
-    apply conv_ref_mrec_bind. rewrite bind_trigger. apply conv_ref_mrec_forall.
-    auto. intros. apply conv_ref_mrec_ret.
-    intros []. rewrite bind_bind. apply conv_ref_mrec_bind.
-    apply conv_ref_mrec_ex. intros. apply conv_ref_mrec_ret.
-    intros n. induction n; cbn.
-    - rewrite bind_ret_l. apply conv_ref_mrec_ex. intros [ | ].
-      2 : apply conv_ref_mrec_spin. apply conv_ref_mrec_bind.
-      + apply conv_ref_mrec_ex. intros. apply conv_ref_mrec_ret.
-      + intros. rewrite bind_bind. setoid_rewrite bind_vis.
-        apply conv_ref_mrec_ex. intros. repeat rewrite bind_ret_l.
-        apply conv_ref_mrec_ret.
-    - rewrite bind_bind. apply conv_ref_mrec_bind; intros; auto.
-      apply conv_ref_mrec_bind.
-      + apply conv_ref_mrec_ex. intros. apply conv_ref_mrec_ret.
-      + intros. rewrite bind_bind. setoid_rewrite bind_vis.
-        apply conv_ref_mrec_ex.
-        intros. repeat rewrite bind_ret_l. pstep. red. cbn.
-        constructor. constructor. auto. left.
-        apply conv_ref_mrec_ret.
-  Qed.
-
-  Lemma prog_ret_spin : forall a, Pre a ->
-                             padded_refines_eq eq (prog a) (partial_spec_fix' a) ->
-                             (exists b, prog a ≈ Ret b) \/ (prog a ≈ ITree.spin).
-  Proof.
-    intros a Href Ha. apply no_ev_to_dec.
-    eapply concrete_conv_ref_padded_to_no_ev; eauto.
-    apply partial_spec_fix_conv_ref. auto.
-  Qed.
-    (* need a padded_refines version *)
-
-(*   Lemma partial_spec_fix_partial_spec' a :
-    (Pre a -> padded_refines_eq eq (prog a) (partial_spec_fix' a)) ->
-    padded_refines_eq eq (prog a) (partial_spec a). *)
-
-
-  Lemma partial_spec_fix_partial_spec_assume_succeed':
-    forall (a : A) (b : B),
-      Pre a ->
-      padded_refines_eq eq (Ret b) (partial_spec_fix' a) ->
-      padded_refines_eq eq (Ret b) (partial_spec a).
-  Proof.
-    intros a b Ha Hfix. unfold partial_spec_fix' in Hfix. cbn in Hfix.
-    repeat setoid_rewrite interp_mrec_spec_or in Hfix.
-
-    (*need an inversion principle for or spec *)
-    (*could use rewrite for interp_mrec_spec and or_spec *)
-    do 2 setoid_rewrite interp_mrec_spec_bind in Hfix. revert Hfix.
-    match goal with | |- context [ interp_mrec_spec ?f _ ] => set f as body end.
-    intro Hfix.
-    assert (
-        padded_refines_eq eq (interp_mrec_spec body (or_spec (b <- exists_spec B;; _ <- assert_spec (Post a b);; Ret b) ITree.spin)) (partial_spec a)).
-    {
-      rewrite interp_mrec_spec_or. unfold partial_spec.
-      apply or_spec_l.
-      - apply or_spec_r. left. unfold total_spec.
-        assumesr. intros. repeat setoid_rewrite interp_mrec_spec_bind.
-        normalize_interp_mrec_spec. setoid_rewrite interp_mrec_spec_ret.
-        setoid_rewrite bind_bind. setoid_rewrite bind_ret_l.
-        eapply padded_refines_bind. reflexivity.
-        intros. subst. eapply padded_refines_bind. reflexivity.
-        intros. subst. reflexivity.
-      - apply or_spec_r. right. rewrite interp_mrec_spec_spin. reflexivity.
-    } setoid_rewrite H in Hfix.
-    setoid_rewrite interp_mrec_spec_ret in Hfix.
-    match type of Hfix with padded_refines_eq eq _ ?t => set t as t1 end.
-    fold t1 in Hfix.
-
-    assert (t1 ≈ (interp_mrec_spec body (trigger (@Spec_forall _ (Pre a))) >>
-                 Ret tt >>
-                  (interp_mrec_spec body
-           (ITree.bind (exists_spec nat)
-              (fun n : nat => trepeat n (ITree.bind (exists_spec A) (fun a' : A =>
-                       trigger (@Spec_exists _ (Pre a')) >> Ret tt >> call_spec a'))))) >> partial_spec a)
-                 ).
-    {
-      unfold t1. repeat rewrite bind_bind.
-      apply eqit_bind. reflexivity. intro.
-      reflexivity.
-    }
-    rewrite H0 in Hfix. clear H0.
-    (*might have dropped an important assumption *)
-    eapply padded_conv_ref_ret_bind; eauto.
-    normalize_interp_mrec_spec. cbn.
-    apply conv_ref_bind.
-    { pstep. red. cbn. constructor; auto. intros a0.
-          left. pstep. red. cbn. constructor. }
-    intros _.  setoid_rewrite bind_ret_l.
-    eapply conv_ref_interp_mrec_conv_ref.
-    Unshelve. 3 : { intros C c. destruct c. apply (Pre a0). }
-    - cbn.
-      intros. destruct d. cbn.
-      clear - H0 Ha. setoid_rewrite bind_bind.
-      apply conv_ref_mrec_bind.
-      { pstep. red. cbn. constructor. auto. left.
-        pstep. constructor. }
-      intros _. rewrite bind_ret_l.
-      repeat rewrite bind_bind. unfold or_spec. setoid_rewrite bind_vis.
-      apply conv_ref_mrec_ex. intros n.
-      rewrite bind_ret_l.
-      eapply conv_ref_mrec_bind.
-      + induction n. cbn. pstep. constructor.
-        cbn. apply conv_ref_mrec_bind; intros; eauto.
-        apply conv_ref_mrec_bind. apply conv_ref_mrec_ex.
-        intros. pstep. constructor. intros.
-        rewrite bind_bind.
-        setoid_rewrite bind_vis.
-        apply conv_ref_mrec_ex. intros Hr.
-        repeat rewrite bind_ret_l. apply conv_ref_mrec_inl.
-        auto. intros. pstep. constructor.
-      + intros []. apply conv_ref_mrec_ex.
-        intros [ | ]; try apply conv_ref_mrec_spin.
-        setoid_rewrite bind_vis. apply conv_ref_mrec_ex.
-        intros. setoid_rewrite bind_ret_l. rewrite bind_bind. setoid_rewrite bind_vis.
-        apply conv_ref_mrec_ex. intros.
-        repeat rewrite bind_ret_l. pstep. constructor.
-    - setoid_rewrite bind_vis. setoid_rewrite bind_ret_l.
-      apply conv_ref_mrec_exists. intros n. clear - n Ha.
-      induction n. cbn. pstep. constructor.
-      cbn. eapply conv_ref_mrec_bind; eauto.
-      setoid_rewrite bind_bind. setoid_rewrite bind_ret_l.
-      setoid_rewrite bind_vis.
-      apply conv_ref_mrec_exists. intros a0. rewrite bind_ret_l.
-      setoid_rewrite bind_vis. apply conv_ref_mrec_exists. intros Ha0.
-      rewrite bind_ret_l. apply conv_ref_mrec_inl. auto. intros. pstep. constructor.
-  Qed.
-
-  Lemma partial_spec_fix_partial_spec_assume_fail a :
-    ~ Pre a -> padded_refines_eq eq (prog a) (partial_spec a).
-  Proof.
-    intros HPre. apply or_spec_r.
-    left. assumesr. intros. contradiction.
-  Qed.
-
-  Lemma partial_spec_fix_partial_spec_assume_succeed:
-    forall (a : A) (b : B),
-      padded_refines_eq eq (Ret b) (partial_spec_fix a) ->
-      padded_refines_eq eq (Ret b) (partial_spec a).
-  Proof.
-    intros a b Hfix.
-    apply or_spec_r. left. unfold total_spec.
-    assumesr. intros Ha.
-    unfold partial_spec_fix in Hfix.
-    do 2 setoid_rewrite interp_mrec_spec_bind in Hfix. revert Hfix.
-    match goal with | |- context [ interp_mrec_spec ?f _ ] => set f as body end.
-    intro Hfix.
-    assert (interp_mrec_spec body (b <- exists_spec B;; _ <- assert_spec (Post a b);; Ret b) ≈
-                             (b <- exists_spec B;; _ <- assert_spec (Post a b);; Ret b)).
-    {
-      repeat setoid_rewrite interp_mrec_spec_bind.
-      normalize_interp_mrec_spec.
-      setoid_rewrite interp_mrec_spec_ret. cbn. reflexivity.
-    } setoid_rewrite H in Hfix.
-    (* need to manage diff between padded_refines and refines *)
-    cbn in Hfix. setoid_rewrite <- bind_bind in Hfix.
-    eapply padded_conv_ref_ret_bind; eauto.
-    setoid_rewrite interp_mrec_spec_ret.
-    apply conv_ref_bind.
-    { pstep. red. cbn. constructor; auto. intros a0.
-          left. pstep. red. cbn. constructor. }
-    intros _.
-    eapply conv_ref_interp_mrec_conv_ref.
-    Unshelve. 3 : { intros C c. destruct c. apply (Pre a0). }
-    - cbn.
-      intros. destruct d. cbn.
-      clear - H0 Ha.
-      repeat rewrite bind_bind. setoid_rewrite bind_ret_l.
-      apply conv_ref_mrec_bind.
-      apply conv_ref_mrec_forall. auto. intros. pstep. constructor.
-      intros. rewrite <- bind_bind.
-      apply conv_ref_mrec_bind.
-      + rewrite bind_bind. apply conv_ref_mrec_bind.
-        apply conv_ref_mrec_exists. intros. pstep. constructor.
-        intros n.
-        induction n; cbn. rewrite bind_ret_l. apply conv_ref_mrec_exists.
-        intros. pstep. constructor. rewrite bind_bind.
-        eapply conv_ref_mrec_bind; intros; eauto.
-        setoid_rewrite bind_vis. apply conv_ref_mrec_exists.
-        intros. setoid_rewrite bind_ret_l. rewrite bind_bind. setoid_rewrite bind_vis.
-        apply conv_ref_mrec_exists. intros. repeat rewrite bind_ret_l.
-        apply conv_ref_mrec_inl. auto. intros. pstep. constructor.
-      + intros b. rewrite bind_bind. setoid_rewrite bind_vis.
-        apply conv_ref_mrec_exists. intros HPost. repeat rewrite bind_ret_l.
-        pstep. constructor.
-    - setoid_rewrite bind_vis. setoid_rewrite bind_ret_l.
-      apply conv_ref_mrec_exists. intros n. clear - n Ha.
-      induction n. cbn. pstep. constructor.
-      cbn. eapply conv_ref_mrec_bind; eauto.
-      setoid_rewrite bind_bind. setoid_rewrite bind_ret_l.
-      setoid_rewrite bind_vis.
-      apply conv_ref_mrec_exists. intros a0. rewrite bind_ret_l.
-      setoid_rewrite bind_vis. apply conv_ref_mrec_exists. intros Ha0.
-      rewrite bind_ret_l. apply conv_ref_mrec_inl. auto. intros. pstep. constructor.
-  Qed.
-
-
-
-  Lemma partial_spec_fix_partial_spec' a :
-    (Pre a -> padded_refines_eq eq (prog a) (partial_spec_fix' a)) ->
-    padded_refines_eq eq (prog a) (partial_spec a).
-  Proof.
-    intros Hfix. destruct (classic (Pre a)).
-    - specialize (Hfix H). apply prog_ret_spin in H as Hdec; auto.
-      destruct Hdec as [ [b Hb] | Hspin ].
-      + rewrite Hb. rewrite Hb in Hfix.
-        apply partial_spec_fix_partial_spec_assume_succeed'; auto.
-      + rewrite Hspin. apply or_spec_r. right. reflexivity.
-    - apply or_spec_r. left. assumesr. intro. contradiction.
-  Qed.
-
-
-  Lemma partial_spec_fix_partial_spec a :
-    (Pre a -> padded_refines_eq eq (prog a) (partial_spec_fix a)) ->
-    padded_refines_eq eq (prog a) (partial_spec a).
-  Proof.
-    intros Hfix. apply partial_spec_fix_partial_spec'.
-    intros Ha. specialize (Hfix Ha). etransitivity; eauto.
-    eapply padded_refines_monot with (RPre1 := eqPreRel) (RPost1 := eqPostRel)
-    (RR1 := eqPostRel _ _ (Call a) (Call a)); auto.
-    { intros. eqPostRel_inv PR. auto. }
-    eapply padded_refines_mrec with (RPreInv := eqPreRel).
-    2 : constructor.
-    intros. eqPreRel_inv H. clear Ha Hfix a. destruct d2.
-    simpl. assumesr. intros Ha. assumesl. auto.
-    repeat rewrite bind_bind.
-    existssl. intros n. existssr n.
-    apply padded_refines_bind with (RR := eq).
-    + apply refl_refines. red. intros. destruct e; do 2 constructor.
-      red. intros. inv H. inj_existT. subst. eqPostRel_inv  H6. auto.
-      inj_existT. subst. eqPostRel_inv H6. auto.
-      auto. apply pad_is_padded.
-    + intros [] [] _ .
-      apply or_spec_r. left. existssl. intros b.
-      existssr b. assertsl. intros. assertsr. auto. apply padded_refines_ret.
-      constructor.
-   Qed.
-
-  Lemma partial_spec_fix_spin' a :
-    padded_refines_eq eq ITree.spin (partial_spec_fix' a).
-  Proof.
-    unfold partial_spec_fix'. setoid_rewrite interp_mrec_spec_bind.
-    repeat normalize_interp_mrec_spec. assumesr. intros.
-    setoid_rewrite interp_mrec_spec_bind.
-    setoid_rewrite interp_mrec_spec_bind.
-    normalize_interp_mrec_spec.
-    match goal with |- context [ interp_mrec_spec ?body_ _  ] => set body_ as body end.
-    setoid_rewrite interp_mrec_exists_spec. existssr 0. cbn.
-    rewrite interp_mrec_spec_ret, bind_ret_l. rewrite interp_mrec_spec_or.
-    apply or_spec_r. right. rewrite interp_mrec_spec_spin. reflexivity.
-  Qed.
-
-
-End SpecFix.
 
 Opaque assume_spec.
 Opaque assert_spec.
@@ -618,92 +150,10 @@ Proof.
     { cbn. repeat rewrite H0. repeat rewrite app_length. lia. }
  Qed.
 
-
-Lemma subEqPreRel_eq_type E P A B (ea : E A) (eb : E B) : subEqPreRel P A B ea eb -> A = B.
-Proof.
-  intros. inv H. auto.
-Qed.
-
-Lemma subEqPreRel_eq E P A (e1 : E A) (e2 : E A) : subEqPreRel P A A e1 e2 -> e1 = e2 /\ P A e1.
-Proof.
-  intros. inv H. inj_existT. subst. auto.
-Qed.
-
-Lemma subEqPostRel_eq_type E P A B (ea : E A) (eb : E B) a b : subEqPostRel P A B ea eb a b -> A = B.
-Proof.
-  intros. inv H. auto.
-Qed.
-
-Lemma subEqPostRel_eq E P A (e1 : E A) (e2 : E A) a1 a2 : subEqPostRel P A A e1 e2 a1 a2 -> e1 = e2 /\ a1 = a2
-                                                                                 /\ P A e1 a1.
-Proof.
-  intros. inv H. inj_existT. subst. auto.
-Qed.
-
-Ltac subEqPreRel_inv H := eapply subEqPreRel_eq_type in H as ?H; subst; eapply subEqPreRel_eq in H as [?H ?H] ; subst.
-Ltac subEqPostRel_inv H := apply subEqPostRel_eq_type in H as ?H; subst; apply subEqPostRel_eq in H as [?H [?H ?H] ]; subst.
-
-
-Global Instance padded_refines_subEqRel E R (RR : R -> R -> Prop) (P1 : forall A, E A -> Prop) (P2 : forall A, E A -> A -> Prop) :
-  Transitive RR ->
-  Transitive (padded_refines (subEqPreRel P1) (subEqPostRel P2) RR).
-Proof.
-  intros HRR t1 t2 t3 Ht12 Ht23. unfold padded_refines in *.
-  eapply refines_monot; try eapply refinesTrans; eauto with solve_padded; try apply pad_is_padded.
-  - intros A B ea eb PR. inv PR. inj_existT. subst. subEqPreRel_inv H3. auto.
-  - intros. subEqPostRel_inv  PR. constructor. intros. destruct H. subEqPreRel_inv H.
-    exists x1. split; constructor; auto.
-  - intros. inv PR. etransitivity; eauto.
-Qed.
-
-Global Instance subEqPostRel_trans E (P : forall A, E A -> A -> Prop) A (e : E A) : Transitive (subEqPostRel P A A e e).
-Proof.
-  intros x y z Hxy Hyz. subEqPostRel_inv Hxy. auto.
-Qed.
-
-(* I think I can save the rest for tomorrow*)
-
-(*
-Global Instance refines_proper_bind_RPre E R RPre RPost S :
-  Proper (@padded_refines E R R eq ==> pointwise_relation _ (padded_refines_eq eq) ==> @padded_refines_eq E S S eq) ITree.bind.
-Proof.
-  repeat intro. subst. unfold padded_refines_eq in *. eapply padded_refines_bind; eauto.
-  intros; subst. auto.
-Qed.
-*)
-
-(*do I need the proper instances? Probably *)
-
-Global Instance  padded_refines_eq_gen E1 E2 R1 R2 RPre RPost RR : Proper (padded_refines_eq eq ==> flip (padded_refines_eq eq) ==> flip impl)
-                                                                (@padded_refines E1 E2 R1 R2 RPre RPost RR).
-Proof.
-  intros t1 t2 Ht12 t3 t4 Ht43. red in Ht43. intro.
-  unfold padded_refines_eq, padded_refines in *. rename H into H24.
-  specialize @refinesTrans with (E1 := E1) (E2 := E1) (E3 := E2) (RPre1 := eqPreRel) (RPre2 := RPre) as Htrans.
-  eapply Htrans in Ht12; eauto; try apply pad_is_padded. clear Htrans.
-  specialize @refinesTrans with (E1 := E1) (E2 := E2) (E3 := E2) (RPre1 := rcomposePreRel eqPreRel RPre) (RPre2 := eqPreRel) as Htrans.
-  eapply Htrans in Ht12; eauto; try apply pad_is_padded. eapply refines_monot; try eapply Ht12.
-  { intros. destruct PR. destruct H. eqPreRel_inv H. eqPreRel_inv H0. auto. }
-  { intros. econstructor. intros. destruct H. eqPreRel_inv H0.
-    inv H. inj_existT. subst. eqPreRel_inv H4. exists x1. split. 2 : constructor.
-    constructor. intros. destruct H. eqPreRel_inv H. exists x0. split; auto. constructor.
-  }
-  { intros. inv PR. inv REL1. auto. }
-Qed.
   (* this is maybe a tad more subtle then I realized, does it require transitivity?,
      that would not be problematic for these relations because there seem to be PER's
 
    *)
-
-Lemma or_spec_bind_l  E1 E2 R1 S R2 RPre RPost RR (t1 t2 : itree_spec E1 S) (k : S -> itree_spec E1 R1) (t3 : itree_spec E2 R2) :
-  padded_refines RPre RPost RR (ITree.bind t1 k) t3 ->
-  padded_refines RPre RPost RR (ITree.bind t2 k) t3 ->
-  padded_refines RPre RPost RR (ITree.bind (or_spec t1 t2) k) t3.
-Proof.
-  unfold padded_refines. intros. setoid_rewrite bind_vis. setoid_rewrite pad_vis.
-  pstep. constructor. intros [ | ]; constructor; pstep_reverse.
-Qed.
-
 
 (*
 Theorem merge
