theories/Combinators.v
@@ -1,0 +1,783 @@
+
+From Coq Require Export Morphisms RelationClasses Setoid Program.Equality.
+From ITree Require Export ITree ITreeFacts Eq.Rutt Props.Finite.
+From Paco Require Import paco.
+From Coq Require Export Eqdep EqdepFacts Logic.Classical.
+Require Import Lia.
+Require Export HeterogeneousEventRelations Refinement ConcreteRefinement ConvergentRefinement.
+
+Import Monads.
+Import MonadNotation.
+Local Open Scope monad_scope.
+Locate MonadNotation.
+Open Scope list_scope.
+
+
+(** * rec_fix_spec *)
+
+Definition call_spec {E A B} (a : A) : itree_spec (callE A B +' E) B :=
+  ITree.trigger (Spec_vis (inl1 (Call a))).
+
+Definition rec_spec {E A B} (body : A -> itree_spec (callE A B +' E) B) (a : A) :
+  itree_spec E B :=
+  mrec_spec (calling' body) (Call a).
+
+Definition rec_fix_spec {E A B}
+(body : (A -> itree_spec (callE A B +' E) B) ->
+        A -> itree_spec (callE A B +' E) B)  :
+  A -> itree_spec E B := rec_spec (body call_spec).
+
+
+(** * assert_spec, assume_spec, exists_spec, forall_spec *)
+
+Definition assert_spec {E} (P : Type) : itree_spec E unit :=
+  trigger (@Spec_exists E P);; Ret tt.
+
+Lemma padded_assert_pad_elim {E1 E2} RPre RPost R1 R2 RR P
+      (phi : itree_spec E1 R1) (kphi : unit -> itree_spec E2 R2) :
+  P -> padded_refines RPre RPost RR phi (kphi tt) ->
+  padded_refines RPre RPost RR phi (ITree.bind (assert_spec P) kphi).
+Proof.
+  intros. setoid_rewrite bind_trigger.
+  unfold padded_refines in *. rewrite pad_bind, pad_vis.
+  setoid_rewrite pad_ret. rewrite bind_vis. setoid_rewrite bind_tau.
+  setoid_rewrite bind_ret_l. pstep. constructor. auto. constructor. pstep_reverse.
+Qed.
+
+Lemma padded_assert_pad_eliml {E1 E2} RPre RPost R1 R2 RR P
+      (phi : itree_spec E1 R1) (kphi : unit -> itree_spec E2 R2) :
+  (P -> padded_refines RPre RPost RR (kphi tt) phi) ->
+  padded_refines RPre RPost RR (ITree.bind (assert_spec P) kphi) phi.
+Proof.
+  intros. setoid_rewrite bind_trigger.
+  unfold padded_refines in *. rewrite pad_bind, pad_vis.
+  setoid_rewrite pad_ret. rewrite bind_vis. setoid_rewrite bind_tau.
+  setoid_rewrite bind_ret_l. pstep. constructor.
+  intros HP. specialize (H HP). constructor. pstep_reverse.
+Qed.
+
+Definition assume_spec {E} (P : Type) : itree_spec E unit :=
+  trigger (@Spec_forall E P);; Ret tt.
+
+Lemma padded_assume_pad_elim {E1 E2} RPre RPost R1 R2 RR P
+      (phi : itree_spec E1 R1) (kphi : unit -> itree_spec E2 R2) :
+  (P -> padded_refines RPre RPost RR phi (kphi tt)) ->
+  padded_refines RPre RPost RR phi (ITree.bind (assume_spec P) kphi).
+Proof.
+  intros. setoid_rewrite bind_trigger.
+  unfold padded_refines in *. rewrite pad_bind, pad_vis.
+  setoid_rewrite pad_ret. rewrite bind_vis. setoid_rewrite bind_tau.
+  setoid_rewrite bind_ret_l. pstep. constructor.
+  intros HP. specialize (H HP). constructor. pstep_reverse.
+Qed.
+
+Lemma padded_assume_pad_eliml {E1 E2} RPre RPost R1 R2 RR P
+      (phi : itree_spec E1 R1) (kphi : unit -> itree_spec E2 R2) :
+  P -> padded_refines RPre RPost RR (kphi tt) phi ->
+  padded_refines RPre RPost RR (ITree.bind (assume_spec P) kphi) phi.
+Proof.
+  intros. setoid_rewrite bind_trigger.
+  unfold padded_refines in *. rewrite pad_bind, pad_vis.
+  setoid_rewrite pad_ret. rewrite bind_vis. setoid_rewrite bind_tau.
+  setoid_rewrite bind_ret_l. pstep. constructor. auto. constructor. pstep_reverse.
+Qed.
+
+Definition exists_spec {E} (T : Type) : itree_spec E T :=
+  trigger (@Spec_exists E T).
+
+(**)
+Lemma exists_spec_elim {E1 E2} S1 R2 S2 RPre RPost RR (phi : itree_spec E1 S1)
+      (kphi : R2 -> itree_spec E2 S2) r :
+  refines RPre RPost RR phi (kphi r) ->
+  refines RPre RPost RR phi (ITree.bind (exists_spec R2) kphi).
+Proof.
+  intros. unfold exists_spec. setoid_rewrite bind_trigger.
+  pstep. econstructor. pstep_reverse.
+Qed.
+
+(*maybe there is a simpler way to derive this proof from the previous one*)
+Lemma padded_exists_spec_elim {E1 E2} S1 R2 S2 RPre RPost RR (phi : itree_spec E1 S1)
+      (kphi : R2 -> itree_spec E2 S2) r :
+  padded_refines RPre RPost RR phi (kphi r) ->
+  padded_refines RPre RPost RR phi (ITree.bind (exists_spec R2) kphi).
+Proof.
+  intros.  unfold padded_refines in *. rewrite pad_bind. setoid_rewrite pad_vis.
+  rewrite bind_vis.
+  setoid_rewrite pad_ret. setoid_rewrite bind_tau. setoid_rewrite bind_ret_l.
+  pstep. econstructor. Unshelve. all : auto. constructor. pstep_reverse.
+Qed.
+
+Lemma padded_exists_spec_eliml {E1 E2} S1 R2 S2 RPre RPost RR (phi : itree_spec E1 S1)
+      (kphi : R2 -> itree_spec E2 S2) :
+  (forall r, padded_refines RPre RPost RR (kphi r) phi) ->
+  padded_refines RPre RPost RR (ITree.bind (exists_spec R2) kphi) phi .
+Proof.
+  intros.  unfold padded_refines in *. rewrite pad_bind. setoid_rewrite pad_vis.
+  rewrite bind_vis.
+  setoid_rewrite pad_ret. setoid_rewrite bind_tau. setoid_rewrite bind_ret_l.
+  pstep. econstructor. intros. constructor. pstep_reverse. apply H.
+Qed.
+
+Ltac existssr a := apply padded_exists_spec_elim with (r := a).
+
+Ltac eexistssr := eapply padded_exists_spec_elim.
+
+Ltac existssl := apply padded_exists_spec_eliml.
+
+Ltac assumesr := apply padded_assume_pad_elim.
+Ltac assumesl := apply padded_assume_pad_eliml.
+Ltac assertsr := apply padded_assert_pad_elim.
+Ltac assertsl := apply padded_assert_pad_eliml.
+
+Lemma conv_ref_exists_spec E R :
+  @conv_ref E R (exists_spec R).
+Proof.
+  pstep. red. cbn. constructor.
+  intros. left. pstep. constructor.
+Qed.
+
+Definition forall_spec {E} (T : Type) : itree_spec E T :=
+  trigger (@Spec_forall E T).
+
+Lemma forall_spec_elim {E1 E2} S1 R2 S2 RPre RPost RR (phi : itree_spec E1 S1)
+      (kphi : R2 -> itree_spec E2 S2) :
+  (forall r, refines RPre RPost RR phi (kphi r)) ->
+  refines RPre RPost RR phi (ITree.bind (forall_spec R2) kphi).
+Proof.
+  intros. unfold forall_spec. rewrite bind_trigger.
+  pstep. constructor. intros. pstep_reverse. apply H.
+Qed.
+
+Lemma padded_forall_spec_elim {E1 E2} S1 R2 S2 RPre RPost RR (phi : itree_spec E1 S1)
+      (kphi : R2 -> itree_spec E2 S2):
+  (forall r, padded_refines RPre RPost RR phi (kphi r)) ->
+  padded_refines RPre RPost RR phi (ITree.bind (forall_spec R2) kphi).
+Proof.
+  intros.  unfold padded_refines in *. rewrite pad_bind. setoid_rewrite pad_vis.
+  rewrite bind_vis.
+  setoid_rewrite pad_ret. setoid_rewrite bind_tau. setoid_rewrite bind_ret_l.
+  pstep. constructor. intros.  constructor. pstep_reverse.
+  apply H.
+Qed.
+
+Lemma padded_forall_spec_eliml {E1 E2} S1 R2 S2 RPre RPost RR (phi : itree_spec E1 S1)
+      (kphi : R2 -> itree_spec E2 S2) r:
+  padded_refines RPre RPost RR (kphi r) phi ->
+  padded_refines RPre RPost RR (ITree.bind (forall_spec R2) kphi) phi.
+Proof.
+  intros.  unfold padded_refines in *. rewrite pad_bind. setoid_rewrite pad_vis.
+  rewrite bind_vis.
+  setoid_rewrite pad_ret. setoid_rewrite bind_tau. setoid_rewrite bind_ret_l.
+  pstep. econstructor. constructor. pstep_reverse.
+Qed.
+
+
+(** * padded_refines_eq *)
+
+Definition padded_refines_eq {E R1 R2} RR (phi1 : itree_spec E R1) (phi2 : itree_spec E R2) :=
+  padded_refines eqPreRel eqPostRel RR phi1 phi2.
+
+Global Instance padded_refines_eq_refl {E R} : Reflexive (@padded_refines_eq E R R eq).
+Proof.
+  red. intros. unfold padded_refines_eq, padded_refines. apply refl_refines; auto.
+  - red. intros. constructor.
+  - red. intros. inv H. inj_existT. subst. auto.
+  - apply pad_is_padded.
+Qed.
+
+Global Instance refines_proper_bind E R S :
+  Proper (@padded_refines_eq E R R eq ==> pointwise_relation _ (padded_refines_eq eq) ==> @padded_refines_eq E S S eq) ITree.bind.
+Proof.
+  repeat intro. subst. unfold padded_refines_eq in *. eapply padded_refines_bind; eauto.
+  intros; subst. auto.
+Qed.
+
+Global Instance refines_proper_subst E R S (k : R -> itree_spec E S) :
+  Proper (@padded_refines_eq E R R eq ==> padded_refines_eq eq) (ITree.subst k).
+Proof.
+  repeat intro. eapply refines_proper_bind. auto. intro. reflexivity.
+Qed.
+
+Global Instance refines_proper_bind_eq E R S :
+  Proper (@padded_refines_eq E R R eq ==> eq ==> @padded_refines_eq E S S eq) ITree.bind.
+Proof.
+  repeat intro. eapply refines_proper_bind. auto. subst. intro. reflexivity.
+Qed.
+
+Global Instance  padded_refines_eq_gen E1 E2 R1 R2 RPre RPost RR :
+  Proper (padded_refines_eq eq ==> flip (padded_refines_eq eq) ==> flip impl)
+         (@padded_refines E1 E2 R1 R2 RPre RPost RR).
+Proof.
+  intros t1 t2 Ht12 t3 t4 Ht43. red in Ht43. intro.
+  unfold padded_refines_eq, padded_refines in *. rename H into H24.
+  specialize @refinesTrans with (E1 := E1) (E2 := E1) (E3 := E2) (RPre1 := eqPreRel) (RPre2 := RPre) as Htrans.
+  eapply Htrans in Ht12; eauto; try apply pad_is_padded. clear Htrans.
+  specialize @refinesTrans with (E1 := E1) (E2 := E2) (E3 := E2) (RPre1 := rcomposePreRel eqPreRel RPre) (RPre2 := eqPreRel) as Htrans.
+  eapply Htrans in Ht12; eauto; try apply pad_is_padded. eapply refines_monot; try eapply Ht12.
+  { intros. destruct PR. destruct H. eqPreRel_inv H. eqPreRel_inv H0. auto. }
+  { intros. econstructor. intros. destruct H. eqPreRel_inv H0.
+    inv H. inj_existT. subst. eqPreRel_inv H4. exists x1. split. 2 : constructor.
+    constructor. intros. destruct H. eqPreRel_inv H. exists x0. split; auto. constructor.
+  }
+  { intros. inv PR. inv REL1. auto. }
+Qed.
+
+Global Instance padded_refines_eq_trans {E R} : Transitive (@padded_refines_eq E R R eq).
+Proof.
+  intros phi1 phi2 phi3 Hphi12 Hphi23. unfold padded_refines_eq, padded_refines in *.
+  eapply refines_monot; try eapply refinesTrans; eauto with solve_padded; try apply pad_is_padded.
+  - intros A B ea eb PR. assert (A = B). inv PR. inv H3. inv H4. auto. subst.
+    assert (ea = eb). inv PR. inj_existT.
+    subst. assert (B = B0). inv H3. auto. subst. inv H4. inj_existT. subst. inv H3. inj_existT.
+    subst. auto. subst. constructor.
+  - intros.
+    assert (A = B). inv PR. auto. subst. assert (ea = eb). inv PR. inj_existT. subst. auto.
+    subst. constructor. intros. destruct H. assert (x0 = x1). inv PR. inj_existT. subst. auto.
+    subst. assert (B = B0). inv H. auto. subst. exists x1.
+    assert (e2 = eb). inv H. inj_existT. subst. auto. subst. repeat constructor.
+  - intros. inv PR. auto.
+Qed.
+
+Global Instance refines_proper_interp_mrec_spec E D R :
+  Proper ((fun ctx1 ctx2 => forall T d, padded_refines_eq  eq (ctx1 T d) (ctx2 T d)) ==> @padded_refines_eq (D +' E) R R eq ==> @padded_refines_eq E R R eq)
+         (fun ctx => @interp_mrec_spec D E ctx R).
+Proof.
+  repeat intro. subst. unfold padded_refines_eq in *.
+  eapply padded_refines_interp_mrec with (RPreInv := eqPreRel) (RPostInv := eqPostRel) ; eauto.
+  - intros.
+    eqPreRel_inv H1.
+    eapply refines_monot; try eapply H.
+    + intros.  eqPreRel_inv PR. destruct x2; repeat constructor.
+    + intros. inv PR; inj_existT; subst; eqPostRel_inv H7; constructor.
+    + intros. subst. constructor.
+  - eapply refines_monot; try eapply H0.
+    + intros. eqPreRel_inv PR. destruct x2; repeat constructor.
+    + intros. inv PR; inj_existT; subst; eqPostRel_inv H7; constructor.
+    + auto.
+Qed.
+
+Global Instance refines_proper_interp_mrec_spec_eq E D R :
+  Proper (eq ==> @padded_refines_eq (D +' E) R R eq ==> @padded_refines_eq E R R eq)
+         (fun ctx => @interp_mrec_spec D E ctx R).
+Proof.
+  repeat intro.
+  apply refines_proper_interp_mrec_spec; auto.
+  intros. subst. reflexivity.
+Qed.
+
+(*
+Global Instance padded_refines_eq_bind_proper  E1 E2 RPre RPost R1 R2 RR :
+  Proper (padded_refines_eq eq ==> eq ==> @padded_refines E1 E2 R1 R2 RPre RPost RR) ITree.bind.
+*)
+(*from there there is a bit more *)
+
+(*need at least bind and ret rules for interp_mrec_spec *)
+
+
+(** * more lemmas about interp_mrec *)
+
+Lemma interp_mrec_ret :
+  forall {D E : Type -> Type} (ctx : forall T : Type, D T -> itree (D +' E) T) R (r :R),
+    interp_mrec ctx (Ret r) ≅ Ret r.
+Proof.
+  intros. setoid_rewrite unfold_iter. cbn. rewrite bind_ret_l. reflexivity.
+Qed.
+
+Lemma interp_mrec_exists_spec E D T (ctx : forall T, D T -> itree_spec (D +' E) T) :
+  interp_mrec_spec ctx (exists_spec T) ≈ exists_spec T.
+Proof.
+  setoid_rewrite interp_mrec_spec'_exists.
+  cbn. apply eqit_Vis. intros.  pstep. red. cbn. constructor. auto.
+Qed.
+
+Lemma interp_mrec_forall_spec E D T (ctx : forall T, D T -> itree_spec (D +' E) T) :
+  interp_mrec_spec ctx (forall_spec T) ≈ forall_spec T.
+Proof.
+  setoid_rewrite interp_mrec_spec'_forall.
+  cbn. apply eqit_Vis. intros.  pstep. red. cbn. constructor. auto.
+Qed.
+
+Lemma interp_mrec_spec_assume E D T (ctx : forall T, D T -> itree_spec (D +' E) T) :
+  interp_mrec_spec ctx (assume_spec T) ≈ assume_spec T.
+Proof.
+  cbn. setoid_rewrite interp_mrec_spec_bind.
+  setoid_rewrite interp_mrec_spec'_forall. rewrite bind_vis, bind_trigger.
+  apply eqit_Vis. intros. setoid_rewrite interp_mrec_spec_ret. rewrite bind_ret_l.
+  reflexivity.
+Qed.
+
+Lemma interp_mrec_spec_assert E D T (ctx : forall T, D T -> itree_spec (D +' E) T) :
+  interp_mrec_spec ctx (assert_spec T) ≈ assert_spec T.
+Proof.
+  cbn. setoid_rewrite interp_mrec_spec_bind.
+  setoid_rewrite interp_mrec_spec'_exists. rewrite bind_vis, bind_trigger.
+  apply eqit_Vis. intros. setoid_rewrite interp_mrec_spec_ret. rewrite bind_ret_l.
+  reflexivity.
+Qed.
+
+Ltac normalize_interp_mrec_spec :=
+  match goal with
+  | |- context [ITree.bind (ITree.bind ?t ?k1) ?k2 ] => setoid_rewrite bind_bind
+  | |- context [interp_mrec_spec ?ctx (ITree.bind ?t ?k) ] => setoid_rewrite interp_mrec_spec_bind
+  | |- context [interp_mrec_spec ?ctx (exists_spec ?T) ] => setoid_rewrite interp_mrec_exists_spec
+  | |- context [interp_mrec_spec ?ctx (forall_spec ?T) ] => setoid_rewrite interp_mrec_forall_spec
+  | |- context [interp_mrec_spec ?ctx (assert_spec ?T) ] => setoid_rewrite interp_mrec_spec_assert
+  | |- context [interp_mrec_spec ?ctx (assume_spec ?T) ] => setoid_rewrite interp_mrec_spec_assume
+  end.
+
+
+(** * or_spec, and_spec *)
+
+Lemma or_spec_l E1 E2 RPre RPost R1 R2 RR (t1 t2 : itree_spec E1 R1) (t3 : itree_spec E2 R2) :
+  @padded_refines E1 E2 R1 R2 RPre RPost RR t1 t3 ->
+  @padded_refines E1 E2 R1 R2 RPre RPost RR t2 t3 ->
+  @padded_refines E1 E2 R1 R2 RPre RPost RR (or_spec t1 t2) t3.
+Proof.
+  intros. unfold or_spec. unfold padded_refines in *.
+  rewrite pad_vis. pstep. constructor. intros [ | ]; constructor; pstep_reverse.
+Qed.
+
+Lemma or_spec_r E1 E2 RPre RPost R1 R2 RR (t1 : itree_spec E1 R1) (t2 t3: itree_spec E2 R2) :
+  (@padded_refines E1 E2 R1 R2 RPre RPost RR t1 t2 \/
+  @padded_refines E1 E2 R1 R2 RPre RPost RR t1 t3) ->
+  @padded_refines E1 E2 R1 R2 RPre RPost RR t1 (or_spec t2 t3).
+Proof.
+  intros. unfold or_spec. unfold padded_refines in *.
+  rewrite pad_vis. pstep.
+  destruct H.
+  - econstructor. constructor. Unshelve. all : try (apply true). pstep_reverse.
+  - econstructor. constructor. Unshelve. all : try (apply false). pstep_reverse.
+Qed.
+
+Lemma interp_mrec_spec_or  (E : Type -> Type) (R : Type) (D : Type -> Type) (ctx : forall T : Type, D T -> itree_spec (D +' E) T)
+  (t1 t2 : itree_spec _ R)
+  : interp_mrec_spec ctx (or_spec t1 t2) ≅ or_spec (interp_mrec_spec ctx t1) (interp_mrec_spec ctx t2).
+Proof.
+  setoid_rewrite interp_mrec_spec'_exists. apply eqit_Vis. intros [ | ]; reflexivity.
+Qed.
+
+(*should be able to generalize this to cany concrete tree *)
+Lemma or_spec_r_Ret_inv E1 E2 R1 R2 RPre RPost RR r t2 t3 :
+  @padded_refines E1 E2 R1 R2 RPre RPost RR (Ret r) (or_spec t2 t3) ->
+  padded_refines RPre RPost RR (Ret r) t2 \/ padded_refines RPre RPost RR (Ret r) t3.
+Proof.
+  intros Hor. unfold padded_refines in *. setoid_rewrite pad_ret in Hor.
+  setoid_rewrite pad_ret. setoid_rewrite pad_vis in Hor.
+  pinversion Hor. inj_existT. subst. inv H1. destruct a.
+  - left. pstep. auto.
+  - right. pstep. auto.
+Qed.
+
+Lemma or_spec_bind_l  E1 E2 R1 S R2 RPre RPost RR (t1 t2 : itree_spec E1 S) (k : S -> itree_spec E1 R1) (t3 : itree_spec E2 R2) :
+  padded_refines RPre RPost RR (ITree.bind t1 k) t3 ->
+  padded_refines RPre RPost RR (ITree.bind t2 k) t3 ->
+  padded_refines RPre RPost RR (ITree.bind (or_spec t1 t2) k) t3.
+Proof.
+  unfold padded_refines. intros. setoid_rewrite bind_vis. setoid_rewrite pad_vis.
+  pstep. constructor. intros [ | ]; constructor; pstep_reverse.
+Qed.
+
+
+(** * spin *)
+
+Lemma spin_bind E R S k : (@ITree.spin E R) >>= k ≅ @ITree.spin E S.
+Proof.
+  ginit. gcofix CIH. gstep. red. cbn. constructor.
+  gfinal. eauto.
+Qed.
+
+Lemma interp_mrec_spec_spin (E : Type -> Type) (R : Type) (D : Type -> Type) (ctx : forall T : Type, D T -> itree_spec (D +' E) T) :
+  interp_mrec_spec ctx ITree.spin ≅ @ITree.spin _ R.
+Proof.
+  pcofix CIH. pstep. red. cbn. constructor.
+  right. eauto.
+Qed.
+
+
+(** * total_spec, partial_spec *)
+
+Lemma padded_refines_ret E1 E2 R1 R2 RPre RPost RR r1 r2 :
+  (RR r1 r2 : Prop) ->
+  @padded_refines E1 E2 R1 R2 RPre RPost RR (Ret r1) (Ret r2).
+Proof.
+  intros Hr. red. repeat rewrite pad_ret. pstep. constructor. auto.
+Qed.
+
+Fixpoint trepeat {E R} (n : nat) (t : itree E R) : itree E unit :=
+  match n with
+  | 0 => Ret tt
+  | S m => t;; trepeat m t end.
+
+Lemma trepeat_Sn E R (n : nat) (t : itree E R) :
+  trepeat (S n) t ≅ t;; trepeat n t.
+Proof.
+  apply eqit_bind; reflexivity.
+Qed.
+
+Lemma trepeat_0 E R (t : itree E R) :
+  trepeat 0 t ≅ Ret tt.
+Proof. reflexivity. Qed.
+
+Section SpecFix.
+  Context {A B: Type} {E : Type -> Type}.
+  Context (Pre : A -> Prop) (Post : A -> B -> Prop).
+  Context (prog : A -> itree_spec E B).
+
+  Context (Rdec : A -> A -> Prop).
+  Context (HRdec : well_founded Rdec).
+
+  Context (Hprog : forall a, isConcrete (prog a)).
+  Variant pre_call : forall C, callE A B C -> Prop :=
+    | pre_call_intro (a : A) : Pre a -> pre_call B (Call a).
+  Variant post_call : forall C, callE A B C -> C -> Prop :=
+    | post_call_intro a b : Post a b -> post_call B (Call a) b.
+
+  Definition total_spec (a : A) : itree_spec E B :=
+    assume_spec (Pre a);;
+    b <- exists_spec B;;
+    assert_spec (Post a b);;
+    Ret b.
+
+  (* better for using as a final spec *)
+  Definition partial_spec (a : A) : itree_spec E B :=
+    or_spec (total_spec a) ITree.spin.
+  (* better for syntax driven solving *)
+  (**)
+
+  Definition partial_spec_fix : A -> itree_spec E B :=
+    rec_fix_spec (fun rec a =>
+                    assume_spec (Pre a);;
+                    (
+                      n <- exists_spec nat;;
+                      trepeat n (a' <- exists_spec A;; assert_spec (Pre a');; rec a')
+                    );;
+                    b <- exists_spec B;;
+                    assert_spec (Post a b);;
+                    Ret b
+                 ).
+
+  Definition partial_spec_fix' : A -> itree_spec E B :=
+    rec_fix_spec (fun rec a =>
+                        assume_spec (Pre a);;
+                        (
+                          n <- exists_spec nat;;
+                          trepeat n (a' <- exists_spec A;; assert_spec (Pre a');; rec a')
+                        );;
+                        or_spec (
+                            b <- exists_spec B;;
+                            assert_spec (Post a b);;
+                            Ret b)
+                        ITree.spin
+                 ).
+
+
+  Definition total_spec_fix : A -> itree_spec E B :=
+    rec_fix_spec (fun rec a =>
+                    assume_spec (Pre a);;
+                    (
+                      n <- exists_spec nat;;
+                      trepeat n (a' <- exists_spec A;; assert_spec (Pre a' /\ Rdec a' a);; rec a')
+                    );;
+                    b <- exists_spec B;;
+                    assert_spec (Post a b);;
+                    Ret b
+                 ).
+
+  (* here would be a good place for proofs that partial_spec_fix' is greater than any of these
+     from there I should be able to prove that total_spec_fix
+   *)
+
+  Lemma total_spec_fix_total a : padded_refines_eq eq (total_spec_fix a) (total_spec a).
+  Proof.
+    revert a.
+    apply well_founded_ind with (R := Rdec). auto.
+    intros a Hind. unfold total_spec_fix. simpl.
+    setoid_rewrite interp_mrec_spec_bind.
+    match goal with |- context [ interp_mrec_spec ?k _ ] => set k as body end.
+    unfold total_spec. assumesr. intros Ha. setoid_rewrite interp_mrec_spec_assume.
+    assumesl. auto. rewrite bind_bind.  setoid_rewrite interp_mrec_spec_bind.
+    setoid_rewrite interp_mrec_exists_spec. existssl. intros n.
+    induction n.
+    - simpl. rewrite bind_ret_l. setoid_rewrite interp_mrec_spec_bind.
+      setoid_rewrite interp_mrec_exists_spec.
+      setoid_rewrite interp_mrec_spec_bind. setoid_rewrite interp_mrec_spec_assert.
+      setoid_rewrite interp_mrec_spec_ret. reflexivity.
+    - simpl. rewrite bind_bind. setoid_rewrite interp_mrec_spec_bind.
+      setoid_rewrite IHn. setoid_rewrite interp_mrec_spec_bind.
+      setoid_rewrite interp_mrec_exists_spec. rewrite bind_bind. existssl.
+      intros a'. setoid_rewrite interp_mrec_spec_bind.
+      setoid_rewrite interp_mrec_spec_assert. rewrite bind_bind. assertsl.
+      intros [Hprea' Hdec]. simpl.
+      assert (Htot : interp_mrec_spec body (call_spec a') ≈ total_spec_fix a').
+      { unfold total_spec_fix, rec_fix_spec, rec_spec, mrec_spec .
+        setoid_rewrite interp_mrec_spec_inl. rewrite tau_eutt. rewrite bind_ret_r.
+        reflexivity. }
+      rewrite Htot, Hind; auto. unfold total_spec.
+      setoid_rewrite bind_bind at 1. assumesl. auto.
+      setoid_rewrite bind_bind at 1. existssl. intros b.
+      setoid_rewrite bind_bind at 1. assertsl. intros. rewrite bind_ret_l. reflexivity.
+   Qed.
+
+
+    Lemma partial_spec_fix_conv_ref :
+    forall a, Pre a -> conv_ref (partial_spec_fix' a).
+  Proof.
+    intros a Ha.
+    eapply conv_ref_mrec_conv_ref with (Pre := pre_call).
+    constructor. auto.
+    intros. inv H. inj_existT. subst.
+    clear a Ha.
+    rename a0 into a. rename H2 into Ha. clear H0. cbn.
+    apply conv_ref_mrec_bind.  rewrite bind_trigger. apply conv_ref_mrec_forall.
+    auto. intros. apply conv_ref_mrec_ret.
+    intros []. rewrite bind_bind. apply conv_ref_mrec_bind.
+    apply conv_ref_mrec_exists. intros. apply conv_ref_mrec_ret.
+    intros n. induction n; cbn.
+    - rewrite bind_ret_l. apply conv_ref_mrec_exists. intros [ | ].
+      2 : apply conv_ref_mrec_spin. apply conv_ref_mrec_bind.
+      + apply conv_ref_mrec_exists. intros. apply conv_ref_mrec_ret.
+      + intros. rewrite bind_bind. setoid_rewrite bind_vis.
+        apply conv_ref_mrec_exists. intros. repeat rewrite bind_ret_l.
+        apply conv_ref_mrec_ret.
+    - rewrite bind_bind. apply conv_ref_mrec_bind; intros; auto.
+      apply conv_ref_mrec_bind.
+      + apply conv_ref_mrec_exists. intros. apply conv_ref_mrec_ret.
+      + intros. rewrite bind_bind. setoid_rewrite bind_vis.
+        apply conv_ref_mrec_exists.
+        intros. repeat rewrite bind_ret_l. pstep. red. cbn.
+        constructor. constructor. auto. left.
+        apply conv_ref_mrec_ret.
+  Qed.
+
+  Lemma prog_ret_spin : forall a, Pre a ->
+                             padded_refines_eq eq (prog a) (partial_spec_fix' a) ->
+                             (exists b, prog a ≈ Ret b) \/ (prog a ≈ ITree.spin).
+  Proof.
+    intros a Href Ha. apply no_ev_to_dec.
+    eapply concrete_conv_ref_padded_to_no_ev; eauto.
+    apply partial_spec_fix_conv_ref. auto.
+  Qed.
+    (* need a padded_refines version *)
+
+(*   Lemma partial_spec_fix_partial_spec' a :
+    (Pre a -> padded_refines_eq eq (prog a) (partial_spec_fix' a)) ->
+    padded_refines_eq eq (prog a) (partial_spec a). *)
+
+
+  Lemma partial_spec_fix_partial_spec_assume_succeed':
+    forall (a : A) (b : B),
+      Pre a ->
+      padded_refines_eq eq (Ret b) (partial_spec_fix' a) ->
+      padded_refines_eq eq (Ret b) (partial_spec a).
+  Proof.
+    intros a b Ha Hfix. unfold partial_spec_fix' in Hfix. cbn in Hfix.
+    repeat setoid_rewrite interp_mrec_spec_or in Hfix.
+
+    (*need an inversion principle for or spec *)
+    (*could use rewrite for interp_mrec_spec and or_spec *)
+    do 2 setoid_rewrite interp_mrec_spec_bind in Hfix. revert Hfix.
+    match goal with | |- context [ interp_mrec_spec ?f _ ] => set f as body end.
+    intro Hfix.
+    assert (
+        padded_refines_eq eq (interp_mrec_spec body (or_spec (b <- exists_spec B;; _ <- assert_spec (Post a b);; Ret b) ITree.spin)) (partial_spec a)).
+    {
+      rewrite interp_mrec_spec_or. unfold partial_spec.
+      apply or_spec_l.
+      - apply or_spec_r. left. unfold total_spec.
+        assumesr. intros. repeat setoid_rewrite interp_mrec_spec_bind.
+        normalize_interp_mrec_spec. setoid_rewrite interp_mrec_spec_ret.
+        setoid_rewrite bind_bind. setoid_rewrite bind_ret_l.
+        eapply padded_refines_bind. reflexivity.
+        intros. subst. eapply padded_refines_bind. reflexivity.
+        intros. subst. reflexivity.
+      - apply or_spec_r. right. rewrite interp_mrec_spec_spin. reflexivity.
+    } setoid_rewrite H in Hfix.
+    setoid_rewrite interp_mrec_spec_ret in Hfix.
+    match type of Hfix with padded_refines_eq eq _ ?t => set t as t1 end.
+    fold t1 in Hfix.
+
+    assert (t1 ≈ (interp_mrec_spec body (trigger (@Spec_forall _ (Pre a))) >>
+                 Ret tt >>
+                  (interp_mrec_spec body
+           (ITree.bind (exists_spec nat)
+              (fun n : nat => trepeat n (ITree.bind (exists_spec A) (fun a' : A =>
+                       trigger (@Spec_exists _ (Pre a')) >> Ret tt >> call_spec a'))))) >> partial_spec a)
+                 ).
+    {
+      unfold t1. repeat rewrite bind_bind.
+      apply eqit_bind. reflexivity. intro.
+      reflexivity.
+    }
+    rewrite H0 in Hfix. clear H0.
+    (*might have dropped an important assumption *)
+    eapply padded_conv_ref_ret_bind; eauto.
+    normalize_interp_mrec_spec. cbn.
+    apply conv_ref_bind.
+    { pstep. red. cbn. constructor; auto. intros a0.
+          left. pstep. red. cbn. constructor. }
+    intros _.  setoid_rewrite bind_ret_l.
+    eapply conv_ref_interp_mrec_conv_ref.
+    Unshelve. 3 : { intros C c. destruct c. apply (Pre a0). }
+    - cbn.
+      intros. destruct d. cbn.
+      clear - H0 Ha. setoid_rewrite bind_bind.
+      apply conv_ref_mrec_bind.
+      { pstep. red. cbn. constructor. auto. left.
+        pstep. constructor. }
+      intros _. rewrite bind_ret_l.
+      repeat rewrite bind_bind. unfold or_spec. setoid_rewrite bind_vis.
+      apply conv_ref_mrec_exists. intros n.
+      rewrite bind_ret_l.
+      eapply conv_ref_mrec_bind.
+      + induction n. cbn. pstep. constructor.
+        cbn. apply conv_ref_mrec_bind; intros; eauto.
+        apply conv_ref_mrec_bind. apply conv_ref_mrec_exists.
+        intros. pstep. constructor. intros.
+        rewrite bind_bind.
+        setoid_rewrite bind_vis.
+        apply conv_ref_mrec_exists. intros Hr.
+        repeat rewrite bind_ret_l. apply conv_ref_mrec_inl.
+        auto. intros. pstep. constructor.
+      + intros []. apply conv_ref_mrec_exists.
+        intros [ | ]; try apply conv_ref_mrec_spin.
+        setoid_rewrite bind_vis. apply conv_ref_mrec_exists.
+        intros. setoid_rewrite bind_ret_l. rewrite bind_bind. setoid_rewrite bind_vis.
+        apply conv_ref_mrec_exists. intros.
+        repeat rewrite bind_ret_l. pstep. constructor.
+    - setoid_rewrite bind_vis. setoid_rewrite bind_ret_l.
+      apply conv_ref_mrec_exists. intros n. clear - n Ha.
+      induction n. cbn. pstep. constructor.
+      cbn. eapply conv_ref_mrec_bind; eauto.
+      setoid_rewrite bind_bind. setoid_rewrite bind_ret_l.
+      setoid_rewrite bind_vis.
+      apply conv_ref_mrec_exists. intros a0. rewrite bind_ret_l.
+      setoid_rewrite bind_vis. apply conv_ref_mrec_exists. intros Ha0.
+      rewrite bind_ret_l. apply conv_ref_mrec_inl. auto. intros. pstep. constructor.
+  Qed.
+
+  Lemma partial_spec_fix_partial_spec_assume_fail a :
+    ~ Pre a -> padded_refines_eq eq (prog a) (partial_spec a).
+  Proof.
+    intros HPre. apply or_spec_r.
+    left. assumesr. intros. contradiction.
+  Qed.
+
+  Lemma partial_spec_fix_partial_spec_assume_succeed:
+    forall (a : A) (b : B),
+      padded_refines_eq eq (Ret b) (partial_spec_fix a) ->
+      padded_refines_eq eq (Ret b) (partial_spec a).
+  Proof.
+    intros a b Hfix.
+    apply or_spec_r. left. unfold total_spec.
+    assumesr. intros Ha.
+    unfold partial_spec_fix in Hfix.
+    do 2 setoid_rewrite interp_mrec_spec_bind in Hfix. revert Hfix.
+    match goal with | |- context [ interp_mrec_spec ?f _ ] => set f as body end.
+    intro Hfix.
+    assert (interp_mrec_spec body (b <- exists_spec B;; _ <- assert_spec (Post a b);; Ret b) ≈
+                             (b <- exists_spec B;; _ <- assert_spec (Post a b);; Ret b)).
+    {
+      repeat setoid_rewrite interp_mrec_spec_bind.
+      normalize_interp_mrec_spec.
+      setoid_rewrite interp_mrec_spec_ret. cbn. reflexivity.
+    } setoid_rewrite H in Hfix.
+    (* need to manage diff between padded_refines and refines *)
+    cbn in Hfix. setoid_rewrite <- bind_bind in Hfix.
+    eapply padded_conv_ref_ret_bind; eauto.
+    setoid_rewrite interp_mrec_spec_ret.
+    apply conv_ref_bind.
+    { pstep. red. cbn. constructor; auto. intros a0.
+          left. pstep. red. cbn. constructor. }
+    intros _.
+    eapply conv_ref_interp_mrec_conv_ref.
+    Unshelve. 3 : { intros C c. destruct c. apply (Pre a0). }
+    - cbn.
+      intros. destruct d. cbn.
+      clear - H0 Ha.
+      repeat rewrite bind_bind. setoid_rewrite bind_ret_l.
+      apply conv_ref_mrec_bind.
+      apply conv_ref_mrec_forall. auto. intros. pstep. constructor.
+      intros. rewrite <- bind_bind.
+      apply conv_ref_mrec_bind.
+      + rewrite bind_bind. apply conv_ref_mrec_bind.
+        apply conv_ref_mrec_exists. intros. pstep. constructor.
+        intros n.
+        induction n; cbn. rewrite bind_ret_l. apply conv_ref_mrec_exists.
+        intros. pstep. constructor. rewrite bind_bind.
+        eapply conv_ref_mrec_bind; intros; eauto.
+        setoid_rewrite bind_vis. apply conv_ref_mrec_exists.
+        intros. setoid_rewrite bind_ret_l. rewrite bind_bind. setoid_rewrite bind_vis.
+        apply conv_ref_mrec_exists. intros. repeat rewrite bind_ret_l.
+        apply conv_ref_mrec_inl. auto. intros. pstep. constructor.
+      + intros b. rewrite bind_bind. setoid_rewrite bind_vis.
+        apply conv_ref_mrec_exists. intros HPost. repeat rewrite bind_ret_l.
+        pstep. constructor.
+    - setoid_rewrite bind_vis. setoid_rewrite bind_ret_l.
+      apply conv_ref_mrec_exists. intros n. clear - n Ha.
+      induction n. cbn. pstep. constructor.
+      cbn. eapply conv_ref_mrec_bind; eauto.
+      setoid_rewrite bind_bind. setoid_rewrite bind_ret_l.
+      setoid_rewrite bind_vis.
+      apply conv_ref_mrec_exists. intros a0. rewrite bind_ret_l.
+      setoid_rewrite bind_vis. apply conv_ref_mrec_exists. intros Ha0.
+      rewrite bind_ret_l. apply conv_ref_mrec_inl. auto. intros. pstep. constructor.
+  Qed.
+
+
+
+  Lemma partial_spec_fix_partial_spec' a :
+    (Pre a -> padded_refines_eq eq (prog a) (partial_spec_fix' a)) ->
+    padded_refines_eq eq (prog a) (partial_spec a).
+  Proof.
+    intros Hfix. destruct (classic (Pre a)).
+    - specialize (Hfix H). apply prog_ret_spin in H as Hdec; auto.
+      destruct Hdec as [ [b Hb] | Hspin ].
+      + rewrite Hb. rewrite Hb in Hfix.
+        apply partial_spec_fix_partial_spec_assume_succeed'; auto.
+      + rewrite Hspin. apply or_spec_r. right. reflexivity.
+    - apply or_spec_r. left. assumesr. intro. contradiction.
+  Qed.
+
+
+  Lemma partial_spec_fix_partial_spec a :
+    (Pre a -> padded_refines_eq eq (prog a) (partial_spec_fix a)) ->
+    padded_refines_eq eq (prog a) (partial_spec a).
+  Proof.
+    intros Hfix. apply partial_spec_fix_partial_spec'.
+    intros Ha. specialize (Hfix Ha). etransitivity; eauto.
+    eapply padded_refines_monot with (RPre1 := eqPreRel) (RPost1 := eqPostRel)
+    (RR1 := eqPostRel _ _ (Call a) (Call a)); auto.
+    { intros. eqPostRel_inv PR. auto. }
+    eapply padded_refines_mrec with (RPreInv := eqPreRel).
+    2 : constructor.
+    intros. eqPreRel_inv H. clear Ha Hfix a. destruct d2.
+    simpl. assumesr. intros Ha. assumesl. auto.
+    repeat rewrite bind_bind.
+    existssl. intros n. existssr n.
+    apply padded_refines_bind with (RR := eq).
+    + apply refl_refines. red. intros. destruct e; do 2 constructor.
+      red. intros. inv H. inj_existT. subst. eqPostRel_inv  H6. auto.
+      inj_existT. subst. eqPostRel_inv H6. auto.
+      auto. apply pad_is_padded.
+    + intros [] [] _ .
+      apply or_spec_r. left. existssl. intros b.
+      existssr b. assertsl. intros. assertsr. auto. apply padded_refines_ret.
+      constructor.
+   Qed.
+
+  Lemma partial_spec_fix_spin' a :
+    padded_refines_eq eq ITree.spin (partial_spec_fix' a).
+  Proof.
+    unfold partial_spec_fix'. setoid_rewrite interp_mrec_spec_bind.
+    repeat normalize_interp_mrec_spec. assumesr. intros.
+    setoid_rewrite interp_mrec_spec_bind.
+    setoid_rewrite interp_mrec_spec_bind.
+    normalize_interp_mrec_spec.
+    match goal with |- context [ interp_mrec_spec ?body_ _  ] => set body_ as body end.
+    setoid_rewrite interp_mrec_exists_spec. existssr 0. cbn.
+    rewrite interp_mrec_spec_ret, bind_ret_l. rewrite interp_mrec_spec_or.
+    apply or_spec_r. right. rewrite interp_mrec_spec_spin. reflexivity.
+  Qed.
+
+
+End SpecFix.
